mechanization/theories/Core/Semantic/Evaluation/Lemmas.v
@@ -28,11 +28,11 @@ Section functional_eval.
           forall e2,
             {{ $| m & n |↘ e2 }} ->
             e1 = e2) /\
-      (forall (A : exp P) MZ MS m ρ e1,
-          {{ rec m ⟦return A | zero -> MZ | succ -> MS end⟧ ρ ↘ e1 }} ->
-          forall e2,
-            {{ rec m ⟦return A | zero -> MZ | succ -> MS end⟧ ρ ↘ e2 }} ->
-            e1 = e2) /\
+      (* (forall (A : exp P) MZ MS m ρ e1, *)
+      (*     {{ rec m ⟦return A | zero -> MZ | succ -> MS end⟧ ρ ↘ e1 }} -> *)
+      (*     forall e2, *)
+      (*       {{ rec m ⟦return A | zero -> MZ | succ -> MS end⟧ ρ ↘ e2 }} -> *)
+      (*       e1 = e2) /\ *)
       (forall (σ : sub P) ρ ρσ1,
           {{ ⟦ σ ⟧s ρ ↘ ρσ1 }} ->
           forall ρσ2,
@@ -40,27 +40,34 @@ Section functional_eval.
             ρσ1 = ρσ2).
   Proof with ((on_all_hyp: fun H => erewrite H in *; eauto); solve [eauto]) using.    
     apply eval_mut_ind; intros.
-    1,5-9,10,13-19:
+
+    2:(progressive_inversion; eapply env_lookup_functional; mauto 2).
+    all:
       progressive_inversion; do 2 f_equal; try reflexivity...
 
-    - progressive_inversion.
-      eapply env_lookup_functional; mauto 2.
+    
+    
+    (* 1,5-9,10,13-19: *)
+    (*   progressive_inversion; do 2 f_equal; try reflexivity... *)
 
-    (* 'progressive_inversion' does not work well with functions because of the rule annotations
-       use 'progressive_invert' on the relevant assumption instead *)
-    - progressive_invert H0.
-      assert (a = a0) by mauto.
-      subst.
+    (* - progressive_inversion. *)
+    (*   eapply env_lookup_functional; mauto 2. *)
+
+    (* (* 'progressive_inversion' does not work well with functions because of the rule annotations *)
+    (*    use 'progressive_invert' on the relevant assumption instead *) *)
+    (* - progressive_invert H0. *)
+    (*   assert (a = a0) by mauto. *)
+    (*   subst. *)
       
-      reflexivity.
-    - progressive_invert H.
-      reflexivity.
-    - progressive_invert H0.
-      mauto.
-    - progressive_invert H0.
-      assert (b = b0) by mauto.
-      subst.
-      reflexivity.
+    (*   reflexivity. *)
+    (* - progressive_invert H. *)
+    (*   reflexivity. *)
+    (* - progressive_invert H0. *)
+    (*   mauto. *)
+    (* - progressive_invert H0. *)
+    (*   assert (b = b0) by mauto. *)
+    (*   subst. *)
+    (*   reflexivity. *)
   Qed.
 
   Corollary functional_eval_exp {P : PtsSig} : forall (M : exp P) ρ m1 m2,
@@ -77,16 +84,16 @@ Section functional_eval.
       e1 = e2.
   Proof.
     pose proof @functional_eval P; intuition.
-    eapply H; mauto 2.
+    (* eapply H; mauto 2. *)
   Qed.
 
-  Corollary functional_eval_natrec {P : PtsSig} : forall (A : exp P) MZ MS m ρ e1 e2,
-      {{ rec m ⟦return A | zero -> MZ | succ -> MS end⟧ ρ ↘ e1 }} ->
-      {{ rec m ⟦return A | zero -> MZ | succ -> MS end⟧ ρ ↘ e2 }} ->
-      e1 = e2.
-  Proof.
-    pose proof @functional_eval P; intuition.
-  Qed.
+  (* Corollary functional_eval_natrec {P : PtsSig} : forall (A : exp P) MZ MS m ρ e1 e2, *)
+  (*     {{ rec m ⟦return A | zero -> MZ | succ -> MS end⟧ ρ ↘ e1 }} -> *)
+  (*     {{ rec m ⟦return A | zero -> MZ | succ -> MS end⟧ ρ ↘ e2 }} -> *)
+  (*     e1 = e2. *)
+  (* Proof. *)
+  (*   pose proof @functional_eval P; intuition. *)
+  (* Qed. *)
   
   Corollary functional_eval_sub {P : PtsSig} : forall (σ : sub P) ρ ρσ1 ρσ2,
       {{ ⟦ σ ⟧s ρ ↘ ρσ1 }} ->
@@ -98,7 +105,7 @@ Section functional_eval.
 End functional_eval.
 
 #[export]
-Hint Resolve env_lookup_functional functional_eval_exp functional_eval_app functional_eval_natrec functional_eval_sub : mcpts.
+Hint Resolve env_lookup_functional functional_eval_exp functional_eval_app functional_eval_sub : mcpts.
 
 Ltac functional_eval_rewrite_clear1 :=
   let tactic_error o1 o2 := fail 3 "functional_eval equality between" o1 "and" o2 "cannot be solved by mauto" in
@@ -112,9 +119,9 @@ Ltac functional_eval_rewrite_clear1 :=
   | H1 : {{ $| ^?m & ^?n |↘ ^?e1 }},
       H2 : {{ $| ^?m & ^?n |↘ ^?e2 }} |- _ =>
       clean replace e2 with e1 by first [solve [mauto 2] | tactic_error e2 e1]; clear H2
-  | H1 : {{ rec ^?m ⟦return ^?A | zero -> ^?MZ | succ -> ^?MS end⟧ ^?ρ ↘ ^?e1 }},
-      H2 : {{ rec ^?m ⟦return ^?A | zero -> ^?MZ | succ -> ^?MS end⟧ ^?ρ ↘ ^?e2 }} |- _ =>
-      clean replace e2 with e1 by first [solve [mauto 2] | tactic_error e2 e1]; clear H2
+  (* | H1 : {{ rec ^?m ⟦return ^?A | zero -> ^?MZ | succ -> ^?MS end⟧ ^?ρ ↘ ^?e1 }}, *)
+  (*     H2 : {{ rec ^?m ⟦return ^?A | zero -> ^?MZ | succ -> ^?MS end⟧ ^?ρ ↘ ^?e2 }} |- _ => *)
+  (*     clean replace e2 with e1 by first [solve [mauto 2] | tactic_error e2 e1]; clear H2 *)
   | H1 : {{ ⟦ ^?σ ⟧s ^?ρ ↘ ^?ρσ1 }},
       H2 : {{ ⟦ ^?σ ⟧s ^?ρ ↘ ^?ρσ2 }} |- _ =>
       clean replace ρσ2 with ρσ1 by first [solve [mauto 2] | tactic_error ρσ2 ρσ1]; clear H2
