mechanization/theories/Core/Semantic/Readback/Lemmas.v
@@ -25,22 +25,24 @@ Section functional_read.
             A1 = A2).
   Proof with (functional_eval_rewrite_clear; f_equal; solve [eauto]) using.
     apply read_mut_ind; intros.
-    1, 3-9,10,12,13: progressive_inversion...
-    - progressive_invert H1.
-      assert (A = A0) by mauto.
-      assert (b = b0) by (eapply functional_eval_exp; mauto).
-      assert (m' = m'0) by (eapply functional_eval_app; mauto).
-      subst.      
-      assert (M = M0) by mauto.
-      subst.
-      reflexivity.
-    - progressive_invert H1.
-      assert (A = A0) by mauto.
-      assert (b = b0) by (eapply functional_eval_exp; mauto).
-      subst.
-      assert (B' = B'0) by mauto.
-      subst.
-      reflexivity.
+    all: progressive_inversion...
+    
+    (* 1, 3-9,10,12,13: progressive_inversion... *)
+    (* - progressive_invert H1. *)
+    (*   assert (A = A0) by mauto. *)
+    (*   assert (b = b0) by (eapply functional_eval_exp; mauto). *)
+    (*   assert (m' = m'0) by (eapply functional_eval_app; mauto). *)
+    (*   subst.       *)
+    (*   assert (M = M0) by mauto. *)
+    (*   subst. *)
+    (*   reflexivity. *)
+    (* - progressive_invert H1. *)
+    (*   assert (A = A0) by mauto. *)
+    (*   assert (b = b0) by (eapply functional_eval_exp; mauto). *)
+    (*   subst. *)
+    (*   assert (B' = B'0) by mauto. *)
+    (*   subst. *)
+    (*   reflexivity. *)
   Qed.
 
   Corollary functional_read_nf {P : PtsSig} : forall i (v : domain_nf P) V1 V2,
