mechanization/theories/Core/Semantic/Realizability.v
@@ -6,17 +6,17 @@ From McPTS.Core Require Import Base.
 From McPTS.Core.Semantic Require Export NbE PER.
 Import Domain_Notations.
 
-Lemma per_nat_then_per_top {P} : forall {n m : domain P},
-    {{ Dom n ≈ m ∈ per_nat }} ->
-    {{ Dom ⇓ ℕ n ≈ ⇓ ℕ m ∈ per_top }}.
-Proof with solve [destruct_conjs; eexists; repeat econstructor; eauto].
-  induction 1; simpl in *; intros s;
-    try specialize (IHper_nat s);
-    try specialize (H s)...
-Qed.
+(* Lemma per_nat_then_per_top {P} : forall {n m : domain P}, *)
+(*     {{ Dom n ≈ m ∈ per_nat }} -> *)
+(*     {{ Dom ⇓ ℕ n ≈ ⇓ ℕ m ∈ per_top }}. *)
+(* Proof with solve [destruct_conjs; eexists; repeat econstructor; eauto]. *)
+(*   induction 1; simpl in *; intros s; *)
+(*     try specialize (IHper_nat s); *)
+(*     try specialize (H s)... *)
+(* Qed. *)
 
-#[export]
-Hint Resolve per_nat_then_per_top : mcpts.
+(* #[export] *)
+(* Hint Resolve per_nat_then_per_top : mcpts. *)
 
 Lemma realize_per_sort_elem_gen {P : PtsSig} {pred_P : PredicativeSig P} : forall {s a a' R},
     {{ DF a ≈ a' ∈ per_sort_elem pred_P s ↘ R }} ->
