mechanization/theories/Core/Syntactic/CoreInversions.v
@@ -5,79 +5,103 @@ From McPTS.Core.Syntactic Require Export CtxEq.
 Import Syntax_Notations.
 
 
-Lemma wf_pi_inversion {P : PtsSig} : forall {Γ : ctx P} {A B C s1 s2 s3} {r : Ru P s1 s2 s3},
-    {{ Γ ⊢ Π r A B : C }} ->
-    {{ Γ ⊢ A : Sort@s1 }} /\ {{ Γ, A ⊢ B : Sort@s2 }} /\ {{ Γ ⊢ Sort@s3 ≈ C }}.
+Lemma wf_pi_inversion {P : PtsSig} : forall {Γ : ctx P} {A B C},
+    {{ Γ ⊢ Π A B : C }} ->
+    exists s1 s2 s3,
+      Ru P s1 s2 s3 /\ {{ Γ ⊢ A : Sort@s1 }} /\ {{ Γ, A ⊢ B : Sort@s2 }} /\ {{ Γ ⊢ Sort@s3 ≈ C }}.
 Proof with mautosolve 4.  
   intros * H.
   dependent induction H;
     gen_core_presups; mauto.
-  split; [|split];
-    [| | transitivity A0; mauto 2];
-    eapply IHwf_exp; mauto 2.
+  - do 3 eexists; repeat split; mauto 3.
+  - specialize (IHwf_exp A B A0).
+    assert (exists s1 s2 s3 : P,
+               Ru P s1 s2 s3 /\
+                 {{ Γ ⊢ A : Sort@s1 }} /\ {{ Γ,A ⊢ B : Sort@s2 }} /\ {{ Γ ⊢ Sort@s3 ≈ A0 }}) by mauto 2.
+    destruct_conjs.
+    do 3 eexists; repeat split; mauto 2.
 Qed.
 
 #[export]
 Hint Resolve wf_pi_inversion : mcpts.
 
 (* I am not sure this is really relevant in our setting *)
-Corollary wf_pi_inversion' {P : PtsSig} : forall {Γ : ctx P} {A B C s1 s2 s3} {r : Ru P s1 s2 s3},
-    {{ Γ ⊢ Π r A B : C }} ->
-    {{ Γ ⊢ A : Sort@s1 }} /\ {{ Γ, A ⊢ B : Sort@s2 }}.
+Corollary wf_pi_inversion' {P : PtsSig} : forall {Γ : ctx P} {A B C},
+    {{ Γ ⊢ Π A B : C }} ->
+    exists s1 s2 s3,
+      Ru P s1 s2 s3 /\ {{ Γ ⊢ A : Sort@s1 }} /\ {{ Γ, A ⊢ B : Sort@s2 }}.
 Proof with mautosolve 4.
   intros.
-  assert ({{ Γ ⊢ A : Sort@s1 }} /\ {{ Γ, A ⊢ B : Sort@s2 }} /\ {{ Γ ⊢ Sort@s3 ≈ C }}) by (eapply wf_pi_inversion; mauto 2).
-  destruct_conjs; mauto 2.
+  assert (exists s1 s2 s3, Ru P s1 s2 s3 /\ {{ Γ ⊢ A : Sort@s1 }} /\ {{ Γ, A ⊢ B : Sort@s2 }} /\ {{ Γ ⊢ Sort@s3 ≈ C }}) by (eapply wf_pi_inversion; mauto 2).
+  destruct_conjs; repeat eexists; mauto 2.
 Qed.
 
-Corollary wf_pi_inversion_typ {P} : forall {Γ : ctx P} {A B C s1 s2 s3} {r : Ru P s1 s2 s3},
-    {{ Γ ⊢ Π r A B : C }} ->
-    {{ Γ ⊢ Sort@s3 ≈ C }}.
+Corollary wf_pi_inversion_typ {P} : forall {Γ : ctx P} {A B C},
+    {{ Γ ⊢ Π A B : C }} ->
+    exists s1 s2 s3, Ru P s1 s2 s3 /\ {{ Γ ⊢ Sort@s3 ≈ C }}.
 Proof.
   intros.
-  assert ({{ Γ ⊢ A : Sort@s1 }} /\ {{ Γ, A ⊢ B : Sort@s2 }} /\ {{ Γ ⊢ Sort@s3 ≈ C }}) by (eapply wf_pi_inversion; mauto 2).
-  destruct_conjs; mauto 2.  
+  assert (exists s1 s2 s3, Ru P s1 s2 s3 /\ {{ Γ ⊢ A : Sort@s1 }} /\ {{ Γ, A ⊢ B : Sort@s2 }} /\ {{ Γ ⊢ Sort@s3 ≈ C }}) by (eapply wf_pi_inversion; mauto 2).
+  destruct_conjs; repeat eexists; mauto 2.  
 Qed.
 
 
 #[export]
 Hint Resolve wf_pi_inversion' wf_pi_inversion_typ : mcpts.
 
-Corollary wf_typ_pi_inversion {P : PtsSig} : forall {Γ : ctx P} {A B s1 s2 s3} {r : Ru P s1 s2 s3},
-    {{ Γ ⊢ Π r A B }} ->
-    {{ Γ ⊢ A : Sort@s1 }} /\ {{ Γ, A ⊢ B : Sort@s2 }}.
+Corollary wf_typ_pi_inversion {P : PtsSig} : forall {Γ : ctx P} {A B},
+    {{ Γ ⊢ Π A B }} ->
+    exists s1 s2 s3, Ru P s1 s2 s3 /\ {{ Γ ⊢ A : Sort@s1 }} /\ {{ Γ, A ⊢ B : Sort@s2 }} /\ {{ Γ ⊢ Π A B : Sort@s3 }}.
 Proof.
-  intros * H; inversion H; mauto 2.
+  intros * H.
+  inversion_clear H.
+  assert (exists s1 s2 s3, Ru P s1 s2 s3 /\ {{ Γ ⊢ A : Sort@s1 }} /\ {{ Γ, A ⊢ B : Sort@s2 }} /\ {{ Γ ⊢ Sort@s3 ≈ Sort@s }}) as [s1 [s2 [s3]]] by mauto 2.
+  destruct_conjs.
+  repeat eexists; mauto 2.
 Qed.
 
 #[export]
 Hint Resolve wf_typ_pi_inversion : mcpts.
 
-Corollary wf_typ_pi_inversion' {P : PtsSig} : forall {Γ : ctx P} {A B s1 s2 s3} {r : Ru P s1 s2 s3},
-    {{ Γ ⊢ Π r A B }} ->
-    {{ Γ ⊢ Π r A B : Sort@s3 }}.
+Corollary wf_typ_pi_inversion' {P : PtsSig} : forall {Γ : ctx P} {A B},
+    {{ Γ ⊢ Π A B }} ->
+    exists s1 s2 s3,
+      Ru P s1 s2 s3 /\ {{ Γ ⊢ A : Sort@s1 }} /\ {{ Γ, A ⊢ B : Sort@s2 }}.
 Proof.
-  intros * H.
-  assert ({{ Γ ⊢ A : Sort@s1 }} /\ {{ Γ, A ⊢ B : Sort@s2 }}) by mauto 2.
-  destruct_conjs.
-  econstructor; mauto 2.
+  intros.
+  assert (exists s1 s2 s3, Ru P s1 s2 s3 /\ {{ Γ ⊢ A : Sort@s1 }} /\ {{ Γ, A ⊢ B : Sort@s2 }} /\ {{ Γ ⊢ Π A B : Sort@s3 }}) by mauto 2.
+  destruct_conjs; repeat eexists; mauto 2.
 Qed.
 
 #[export]
 Hint Resolve wf_typ_pi_inversion' : mcpts.
 
+Corollary wf_typ_pi_inversion_typ {P} : forall {Γ : ctx P} {A B},
+    {{ Γ ⊢ Π A B }} ->
+    exists s1 s2 s3,
+      Ru P s1 s2 s3 /\ {{ Γ ⊢ Π A B : Sort@s3 }}.
+Proof.
+  intros.
+  assert (exists s1 s2 s3, Ru P s1 s2 s3 /\ {{ Γ ⊢ A : Sort@s1 }} /\ {{ Γ, A ⊢ B : Sort@s2 }} /\ {{ Γ ⊢ Π A B : Sort@s3 }}) by mauto 2.
+  destruct_conjs; repeat eexists; mauto 2.
+Qed.
 
-Corollary wf_fn_inversion {P : PtsSig} : forall {Γ : ctx P} {A M C s1 s2 s3} {r : Ru P s1 s2 s3},
-    {{ Γ ⊢ λ r A M : C }} ->
-    exists B, {{ Γ, A ⊢ M : B }} /\ {{ Γ ⊢ Π r A B ≈ C }}.
+#[export]
+Hint Resolve wf_typ_pi_inversion_typ : mcpts.
+
+
+Corollary wf_fn_inversion {P : PtsSig} : forall {Γ : ctx P} {A M C},
+    {{ Γ ⊢ λ A M : C }} ->
+    exists s1 s2 s3 B, Ru P s1 s2 s3 /\ {{ Γ, A ⊢ M : B }} /\ {{ Γ ⊢ Π A B ≈ C }}.
 Proof with solve [mauto].
   intros * H.
   dependent induction H;
     gen_core_presups.
-  - eexists; split; mauto.
-  - assert (exists B, {{ Γ, A ⊢ M : B }} /\ {{ Γ ⊢ Π r A B ≈ A0 }}) by (eapply IHwf_exp; mauto).
+  - repeat eexists; mauto.
+  - specialize (IHwf_exp A M A0).
+    assert (exists s1 s2 s3 B, Ru P s1 s2 s3 /\ {{ Γ, A ⊢ M : B }} /\ {{ Γ ⊢ Π A B ≈ A0 }}) by mauto 2.
   destruct_conjs.
-  eexists; split; mauto.
+  repeat eexists; mauto.
 Qed.
 
 #[export]
@@ -85,18 +109,19 @@ Hint Resolve wf_fn_inversion : mcpts.
 
 Lemma wf_app_inversion {P : PtsSig} : forall {Γ : ctx P} {M N C},
     {{ Γ ⊢ M N : C }} ->
-    exists A B s1 s2 s3 (r : Ru P s1 s2 s3), {{ Γ ⊢ M : Π r A B }} /\ {{ Γ ⊢ N : A }} /\ {{ Γ ⊢ B[Id,,N] ≈ C }}.
+    exists A B s1 s2 s3, Ru P s1 s2 s3 /\ {{ Γ ⊢ M : Π A B }} /\ {{ Γ ⊢ N : A }} /\ {{ Γ ⊢ B[Id,,N] ≈ C }}.
 Proof with mautosolve 4.
   intros * H.
   dependent induction H;
     gen_core_presups.
   - do 6 eexists; repeat split; eauto.
     eapply wf_typ_eq_refl.
-    assert {{ Γ ⊢ Π r A B : Sort@s3 }} by mauto.
+    assert {{ Γ ⊢ Π A B : Sort@s3 }} by mauto.
     assert ({{ Γ ⊢ A : Sort@s1 }} /\ {{ Γ, A ⊢ B : Sort@s2 }}) by mauto.
     destruct_conjs.
     econstructor; mauto 3.
-  - assert (exists A0 B s1 s2 s3 r, {{ Γ ⊢ M : Π r A0 B }} /\ {{ Γ ⊢ N : A0 }} /\ {{ Γ ⊢ B[Id,,N] ≈ A }}) by (eapply IHwf_exp; mauto).
+  - 
+    assert (exists A0 B s1 s2 s3, Ru P s1 s2 s3 /\ {{ Γ ⊢ M : Π A0 B }} /\ {{ Γ ⊢ N : A0 }} /\ {{ Γ ⊢ B[Id,,N] ≈ A }}) by (eapply IHwf_exp; mauto).
     destruct_conjs.
     do 6 eexists; repeat split; mauto.  
 Qed.
@@ -120,74 +145,74 @@ Qed.
 #[export]
 Hint Resolve wf_vlookup_inversion : mcpts.
 
-Lemma wf_nat_inversion {P} : forall {Γ : ctx P} {A},
-    {{ Γ ⊢ ℕ : A }} ->
-    exists s (r : Ru_nat P s),
-      {{ Γ ⊢ Sort@s ≈ A }}.
-Proof with mautosolve.
-  intros * H.
-  dependent induction H.
-  - eexists. mauto.
-  - specialize (IHwf_exp A0 ltac:(reflexivity) ltac:(reflexivity)).
-    destruct_conjs.
-    do 2 eexists. apply H2.
-    etransitivity; mauto.
-Qed.
+(* Lemma wf_nat_inversion {P} : forall {Γ : ctx P} {A}, *)
+(*     {{ Γ ⊢ ℕ : A }} -> *)
+(*     exists s (r : Ru_nat P s), *)
+(*       {{ Γ ⊢ Sort@s ≈ A }}. *)
+(* Proof with mautosolve. *)
+(*   intros * H. *)
+(*   dependent induction H. *)
+(*   - eexists. mauto. *)
+(*   - specialize (IHwf_exp A0 ltac:(reflexivity) ltac:(reflexivity)). *)
+(*     destruct_conjs. *)
+(*     do 2 eexists. apply H2. *)
+(*     etransitivity; mauto. *)
+(* Qed. *)
 
-#[export]
-  Hint Resolve wf_nat_inversion : mcpts.
+(* #[export] *)
+(*   Hint Resolve wf_nat_inversion : mcpts. *)
 
-Corollary wf_zero_inversion {P} : forall {Γ : ctx P} {A},
-    {{ Γ ⊢ zero : A }} ->
-    exists s (r : Ru_nat P s),
-      {{ Γ ⊢ ℕ ≈ A }}.
-Proof with mautosolve.
-  intros * H.
-  dependent induction H.
-  - eexists. mauto.
-  - specialize (IHwf_exp A0 ltac:(reflexivity) ltac:(reflexivity)).
-    destruct_conjs.
-    do 2 eexists. apply H2.
-    etransitivity; mauto.
-Qed.
+(* Corollary wf_zero_inversion {P} : forall {Γ : ctx P} {A}, *)
+(*     {{ Γ ⊢ zero : A }} -> *)
+(*     exists s (r : Ru_nat P s), *)
+(*       {{ Γ ⊢ ℕ ≈ A }}. *)
+(* Proof with mautosolve. *)
+(*   intros * H. *)
+(*   dependent induction H. *)
+(*   - eexists. mauto. *)
+(*   - specialize (IHwf_exp A0 ltac:(reflexivity) ltac:(reflexivity)). *)
+(*     destruct_conjs. *)
+(*     do 2 eexists. apply H2. *)
+(*     etransitivity; mauto. *)
+(* Qed. *)
 
-#[export]
-Hint Resolve wf_zero_inversion : mcpts.
+(* #[export] *)
+(* Hint Resolve wf_zero_inversion : mcpts. *)
 
-Corollary wf_succ_inversion {P} : forall {Γ : ctx P} {A M},
-    {{ Γ ⊢ succ M : A }} ->
-    {{ Γ ⊢ M : ℕ }} /\ {{ Γ ⊢ ℕ ≈ A }}.
-Proof with mautosolve.
-  intros * H.
-  dependent induction H.
-  - eexists; mautosolve.
-  - specialize (IHwf_exp A0 M ltac:(reflexivity) ltac:(reflexivity)).
-    destruct_conjs.
-    eexists. apply H2.
-    etransitivity; mauto.
-Qed.
+(* Corollary wf_succ_inversion {P} : forall {Γ : ctx P} {A M}, *)
+(*     {{ Γ ⊢ succ M : A }} -> *)
+(*     {{ Γ ⊢ M : ℕ }} /\ {{ Γ ⊢ ℕ ≈ A }}. *)
+(* Proof with mautosolve. *)
+(*   intros * H. *)
+(*   dependent induction H. *)
+(*   - eexists; mautosolve. *)
+(*   - specialize (IHwf_exp A0 M ltac:(reflexivity) ltac:(reflexivity)). *)
+(*     destruct_conjs. *)
+(*     eexists. apply H2. *)
+(*     etransitivity; mauto. *)
+(* Qed. *)
 
-#[export]
-Hint Resolve wf_succ_inversion : mcpts.
+(* #[export] *)
+(* Hint Resolve wf_succ_inversion : mcpts. *)
 
-Lemma wf_natrec_inversion {P} : forall {Γ : ctx P} {A M A' MZ MS},
-    {{ Γ ⊢ rec M return A' | zero -> MZ | succ -> MS end : A }} ->
-    {{ Γ ⊢ MZ : A'[Id,,zero] }} /\ {{ Γ, ℕ, A' ⊢ MS : A'[Wk∘Wk,,succ(#1)] }} /\ {{ Γ ⊢ M : ℕ }} /\ {{ Γ ⊢ A'[Id,,M] ≈ A }}.
-Proof with mautosolve.
-  intros * H.
-  dependent induction H.
-  - do 3 (eexists; mauto).
-    eapply wf_typ_eq_refl.
-    assert {{ Γ, ℕ ⊢ A' }}; mauto 2.
-    assert {{ Γ ⊢s Id,,M : Γ, ℕ }} by mauto 4.
-    mauto 2.
-  - specialize (IHwf_exp A0 M A' MZ MS ltac:(reflexivity) ltac:(reflexivity)).
-    destruct_conjs.
-    repeat split; mauto.
-Qed.
+(* Lemma wf_natrec_inversion {P} : forall {Γ : ctx P} {A M A' MZ MS}, *)
+(*     {{ Γ ⊢ rec M return A' | zero -> MZ | succ -> MS end : A }} -> *)
+(*     {{ Γ ⊢ MZ : A'[Id,,zero] }} /\ {{ Γ, ℕ, A' ⊢ MS : A'[Wk∘Wk,,succ(#1)] }} /\ {{ Γ ⊢ M : ℕ }} /\ {{ Γ ⊢ A'[Id,,M] ≈ A }}. *)
+(* Proof with mautosolve. *)
+(*   intros * H. *)
+(*   dependent induction H. *)
+(*   - do 3 (eexists; mauto). *)
+(*     eapply wf_typ_eq_refl. *)
+(*     assert {{ Γ, ℕ ⊢ A' }}; mauto 2. *)
+(*     assert {{ Γ ⊢s Id,,M : Γ, ℕ }} by mauto 4. *)
+(*     mauto 2. *)
+(*   - specialize (IHwf_exp A0 M A' MZ MS ltac:(reflexivity) ltac:(reflexivity)). *)
+(*     destruct_conjs. *)
+(*     repeat split; mauto. *)
+(* Qed. *)
     
-#[export]
-Hint Resolve wf_natrec_inversion : mcpts.
+(* #[export] *)
+(* Hint Resolve wf_natrec_inversion : mcpts. *)
 
 Lemma wf_exp_sub_inversion {P : PtsSig} : forall {Γ : ctx P} {M σ A},
     {{ Γ ⊢ M[σ] : A }} ->
