mechanization/theories/Core/Syntactic/Presup.v
@@ -4,7 +4,7 @@ From McPTS.Core.Syntactic Require Export CtxEq.
 Import Syntax_Notations.
 
 
-Lemma presup_exp_eq_fn_cong_right {P : PtsSig} : forall {Γ : ctx P} {s1 A A' s2 B M' s3} (r : Ru P s1 s2 s3),
+Lemma presup_exp_eq_fn_cong_right {P : PtsSig} : forall {Γ : ctx P} {s1 A A' s2 B M' s3} {r : Ru P s1 s2 s3},
     {{ ⊢ Γ }} ->
     {{ Γ ⊢ A : Sort@s1 }} ->
     {{ Γ ⊢ A' : Sort@s1 }} ->
@@ -12,15 +12,15 @@ Lemma presup_exp_eq_fn_cong_right {P : PtsSig} : forall {Γ : ctx P} {s1 A A' s2
     {{ ⊢ Γ, A }} ->
     {{ Γ, A ⊢ B : Sort@s2 }} ->
     {{ Γ, A ⊢ M' : B }} ->
-    {{ Γ ⊢ λ r A' M' : Π r A B }}.
+    {{ Γ ⊢ λ A' M' : Π A B }}.
 Proof.
   intros.
-  assert {{ Γ ⊢ Π r A B ≈ Π r A' B : Sort@s3 }} by mauto 3.
+  assert {{ Γ ⊢ Π A B ≈ Π A' B : Sort@s3 }} by mauto 3.
   assert {{ Γ ⊢ A ≈ A' }} by mauto 2.
   assert {{ ⊢ Γ, A ≈ Γ, A' }} by (econstructor; mauto 3).
   assert {{ Γ, A' ⊢ M' : B }} by mauto 4.
-  assert {{ Γ ⊢ Π r A B : Sort@s3 }} by mauto 2.
-  enough {{ Γ ⊢ λ r A' M' : Π r A' B }}; mauto.
+  assert {{ Γ ⊢ Π A B : Sort@s3 }} by mauto 2.
+  enough {{ Γ ⊢ λ A' M' : Π A' B }}; mauto.
 Qed.
 
 #[local]
@@ -34,15 +34,15 @@ Lemma presup_exp_eq_fn_sub_right {P : PtsSig} : forall {Γ : ctx P} {σ Δ s1 A 
     {{ ⊢ Δ, A }} ->
     {{ Δ, A ⊢ B : Sort@s2 }} ->
     {{ Δ, A ⊢ M : B }} ->
-    {{ Γ ⊢ λ r A[σ] M[q σ] : (Π r A B)[σ] }}.
+    {{ Γ ⊢ λ A[σ] M[q σ] : (Π A B)[σ] }}.
 Proof.
   intros.
   assert {{ Γ ⊢ A[σ] : Sort@s1 }} by mauto 2.  
   assert {{ Γ, A[σ] ⊢ B[q σ] : Sort@s2 }} by mauto 4.
-  assert {{ Γ ⊢ Π r A[σ] B[q σ] : Sort@s3 }} by mauto 2.
-  assert {{ Γ ⊢ Π r A[σ] B[q σ] ≈ Π r A[σ] B[q σ] : Sort@s3 }} by mauto 2.
+  assert {{ Γ ⊢ Π A[σ] B[q σ] : Sort@s3 }} by mauto 2.
+  assert {{ Γ ⊢ Π A[σ] B[q σ] ≈ Π A[σ] B[q σ] : Sort@s3 }} by mauto 2.
   assert {{ Γ, A[σ] ⊢ M[q σ] : B[q σ] }} by mauto 4.
-  assert {{ Γ ⊢ λ r A[σ] M[q σ] : Π r A[σ] B[q σ] }} by mauto 3.
+  assert {{ Γ ⊢ λ A[σ] M[q σ] : Π A[σ] B[q σ] }} by mauto 3.
   eapply wf_conv; mauto 4.
 Qed.
 
@@ -54,7 +54,7 @@ Lemma presup_exp_eq_app_cong_right {P : PtsSig} : forall {Γ : ctx P} {s1 A B M'
     {{ Γ ⊢ A : Sort@s1 }} ->
     {{ ⊢ Γ, A }} ->
     {{ Γ, A ⊢ B : Sort@s2 }} ->
-    {{ Γ ⊢ M' : Π r A B }} ->
+    {{ Γ ⊢ M' : Π A B }} ->
     {{ Γ ⊢ N : A }} ->
     {{ Γ ⊢ N' : A }} ->
     {{ Γ ⊢ N ≈ N' : A }} ->
@@ -80,15 +80,15 @@ Lemma presup_exp_eq_app_sub_left {P : PtsSig} : forall {Γ : ctx P} {σ Δ s1 A 
     {{ Δ ⊢ A : Sort@s1 }} ->
     {{ ⊢ Δ, A }} ->
     {{ Δ, A ⊢ B : Sort@s2 }} ->
-    {{ Δ ⊢ M : Π r A B }} ->
+    {{ Δ ⊢ M : Π A B }} ->
     {{ Δ ⊢ N : A }} ->
     {{ Γ ⊢ (M N)[σ] : B[σ,,N[σ]] }}.
 Proof.
   intros.
   assert {{ Γ, A[σ] ⊢s q σ : Δ, A }} by mauto 3.
-  assert {{ Γ ⊢ M[σ] : (Π r A B)[σ] }} by mauto 3.
-  assert {{ Γ ⊢ Π r A[σ] B[q σ] : Sort@s3 }} by mauto 4.
-  assert {{ Γ ⊢ M[σ] : Π r A[σ] B[q σ] }} by mauto.
+  assert {{ Γ ⊢ M[σ] : (Π A B)[σ] }} by mauto 3.
+  assert {{ Γ ⊢ Π A[σ] B[q σ] : Sort@s3 }} by mauto 4.
+  assert {{ Γ ⊢ M[σ] : Π A[σ] B[q σ] }} by mauto.
   assert {{ Δ ⊢ N : A[Id] }} by mauto 3.
   assert {{ Γ ⊢s (Id,,N)∘σ ≈ Id∘σ,,N[σ] : Δ, A }} by mauto 4.
   assert {{ Γ ⊢s (Id,,N)∘σ ≈ σ,,N[σ] : Δ, A }} by mauto 3.
@@ -112,7 +112,7 @@ Lemma presup_exp_eq_app_sub_right {P : PtsSig} : forall {Γ : ctx P} {σ Δ s1 A
     {{ Δ ⊢ A : Sort@s1 }} ->
     {{ ⊢ Δ, A }} ->
     {{ Δ, A ⊢ B : Sort@s2 }} ->
-    {{ Δ ⊢ M : Π r A B }} ->
+    {{ Δ ⊢ M : Π A B }} ->
     {{ Δ ⊢ N : A }} ->
     {{ Γ ⊢ M[σ] N[σ] : B[σ,,N[σ]] }}.
 Proof.
@@ -120,7 +120,7 @@ Proof.
   assert {{ Γ ⊢ A[σ] : Sort@s1 }} by mauto 2.
   assert {{ Γ, A[σ] ⊢s q σ : Δ, A }} by mauto 3.
   assert {{ Γ, A[σ] ⊢ B[q σ] : Sort@s2 }} by mauto 2.
-  assert {{ Γ ⊢ M[σ] : Π r A[σ] B[q σ] }} by (eapply wf_conv; mauto 3).
+  assert {{ Γ ⊢ M[σ] : Π A[σ] B[q σ] }} by (eapply wf_conv; mauto 3).
   assert {{ Γ ⊢ N[σ] : A[σ] }} by mauto 2.
   assert {{ Γ ⊢s q σ∘(Id,,N[σ]) ≈ σ,,N[σ] : Δ, A }} by mauto 3.
   assert {{ Γ ⊢s Id,,N[σ] : Γ, A[σ] }} by mauto 3.
@@ -140,15 +140,15 @@ Lemma presup_exp_eq_pi_eta_right {P : PtsSig} : forall {Γ : ctx P} {s1 A B M s2
     {{ Γ ⊢ A : Sort@s1 }} ->
     {{ ⊢ Γ, A }} ->
     {{ Γ, A ⊢ B : Sort@s2 }} ->
-    {{ Γ ⊢ M : Π r A B }} ->
-    {{ Γ ⊢ λ r A (M[Wk] #0) : Π r A B }}.
+    {{ Γ ⊢ M : Π A B }} ->
+    {{ Γ ⊢ λ A (M[Wk] #0) : Π A B }}.
 Proof.
   intros.
   assert {{ Γ, A ⊢s Wk : Γ }} by mauto 2.
   assert {{ Γ, A, A[Wk] ⊢s q Wk : Γ, A }} by mauto 3.
   assert {{ Γ, A ⊢ A[Wk] : Sort@s1 }} by mauto 2.
   assert {{ Γ, A, A[Wk] ⊢ B[q Wk] : Sort@s2 }} by mauto 2.
-  assert {{ Γ, A ⊢ M[Wk] : Π r A[Wk] B[q Wk] }} by (eapply wf_conv; mauto 3).
+  assert {{ Γ, A ⊢ M[Wk] : Π A[Wk] B[q Wk] }} by (eapply wf_conv; mauto 3).
   assert {{ Γ, A ⊢ A[Wk] }} by mauto 3.
   assert {{ Γ, A ⊢ #0 : A[Wk] }} by mauto 2.
   assert {{ Γ, A ⊢s q Wk∘(Id,,#0) ≈ Id : Γ, A }} by (etransitivity; mauto 3).
@@ -320,172 +320,172 @@ Qed.
 #[local]
   Hint Resolve presup_exp_eq_sub_compose_right : mcpts.
 
-Lemma presup_exp_eq_natrec_cong_right {P} : forall {Γ : ctx P} {A A' MZ' MS' M M' s s'} {r : Ru_nat P s},
-    {{ ⊢ Γ, ℕ }} ->
-    {{ Γ, ℕ ⊢ A : Sort@s' }} ->
-    {{ Γ, ℕ ⊢ A' : Sort@s' }} ->
-    {{ Γ, ℕ ⊢ A ≈ A' }} ->
-    {{ ⊢ Γ }} ->
-    {{ Γ ⊢ MZ' : A[Id,,zero] }} ->
-    {{ ⊢ Γ, ℕ, A }} ->
-    {{ Γ, ℕ, A ⊢ MS' : A[Wk∘Wk,,succ #1] }} ->
-    {{ ⊢ Γ }} ->
-    {{ Γ ⊢ M : ℕ }} ->
-    {{ Γ ⊢ M' : ℕ }} ->
-    {{ Γ ⊢ M ≈ M' : ℕ }} ->
-    {{ Γ ⊢ rec M' return A' | zero -> MZ' | succ -> MS' end : A[Id,,M] }}.
-Proof.
-  intros.
-  assert {{ Γ, ℕ ⊢ A }} by mauto 3.
-  assert {{ Γ, ℕ ⊢ A' }} by mauto 3.
-  assert {{ Γ ⊢s Id,,M : Γ, ℕ }} by mauto 3.
-  assert {{ Γ ⊢s Id,,M' : Γ, ℕ }} by mauto 3.
-  assert {{ Γ ⊢s Id,,M ≈ Id,,M' : Γ, ℕ }} by mauto 3.
-  assert {{ Γ ⊢ A[Id,,M] ≈ A'[Id,,M'] }} by (transitivity {{{ A[Id,,M'] }}}; mauto).
-  assert {{ Γ ⊢s Id,,zero : Γ, ℕ }} by mauto 4.
-  assert {{ Γ ⊢ MZ' : A'[Id,,zero] }} by mauto 4.
-  assert {{ Γ, ℕ, A ⊢s Wk∘Wk,,succ #1 : Γ, ℕ }} by (eapply @sub_weak_compose_weak_extend_succ_var_1 with (P := P); mauto).
+(* Lemma presup_exp_eq_natrec_cong_right {P} : forall {Γ : ctx P} {A A' MZ' MS' M M' s s'} {r : Ru_nat P s}, *)
+(*     {{ ⊢ Γ, ℕ }} -> *)
+(*     {{ Γ, ℕ ⊢ A : Sort@s' }} -> *)
+(*     {{ Γ, ℕ ⊢ A' : Sort@s' }} -> *)
+(*     {{ Γ, ℕ ⊢ A ≈ A' }} -> *)
+(*     {{ ⊢ Γ }} -> *)
+(*     {{ Γ ⊢ MZ' : A[Id,,zero] }} -> *)
+(*     {{ ⊢ Γ, ℕ, A }} -> *)
+(*     {{ Γ, ℕ, A ⊢ MS' : A[Wk∘Wk,,succ #1] }} -> *)
+(*     {{ ⊢ Γ }} -> *)
+(*     {{ Γ ⊢ M : ℕ }} -> *)
+(*     {{ Γ ⊢ M' : ℕ }} -> *)
+(*     {{ Γ ⊢ M ≈ M' : ℕ }} -> *)
+(*     {{ Γ ⊢ rec M' return A' | zero -> MZ' | succ -> MS' end : A[Id,,M] }}. *)
+(* Proof. *)
+(*   intros. *)
+(*   assert {{ Γ, ℕ ⊢ A }} by mauto 3. *)
+(*   assert {{ Γ, ℕ ⊢ A' }} by mauto 3. *)
+(*   assert {{ Γ ⊢s Id,,M : Γ, ℕ }} by mauto 3. *)
+(*   assert {{ Γ ⊢s Id,,M' : Γ, ℕ }} by mauto 3. *)
+(*   assert {{ Γ ⊢s Id,,M ≈ Id,,M' : Γ, ℕ }} by mauto 3. *)
+(*   assert {{ Γ ⊢ A[Id,,M] ≈ A'[Id,,M'] }} by (transitivity {{{ A[Id,,M'] }}}; mauto). *)
+(*   assert {{ Γ ⊢s Id,,zero : Γ, ℕ }} by mauto 4. *)
+(*   assert {{ Γ ⊢ MZ' : A'[Id,,zero] }} by mauto 4. *)
+(*   assert {{ Γ, ℕ, A ⊢s Wk∘Wk,,succ #1 : Γ, ℕ }} by (eapply @sub_weak_compose_weak_extend_succ_var_1 with (P := P); mauto). *)
     
-  assert {{ Γ, ℕ, A ⊢ MS' : A'[Wk∘Wk,,succ #1] }} by mauto 4.
-  assert {{ ⊢ Γ, ℕ, A ≈ Γ, ℕ, A' }} by mauto 3.
-  assert {{ Γ, ℕ, A' ⊢ MS' : A'[Wk∘Wk,,succ #1] }} by mauto 3.
-  eapply wf_conv; mauto 2.
-Qed.
+(*   assert {{ Γ, ℕ, A ⊢ MS' : A'[Wk∘Wk,,succ #1] }} by mauto 4. *)
+(*   assert {{ ⊢ Γ, ℕ, A ≈ Γ, ℕ, A' }} by mauto 3. *)
+(*   assert {{ Γ, ℕ, A' ⊢ MS' : A'[Wk∘Wk,,succ #1] }} by mauto 3. *)
+(*   eapply wf_conv; mauto 2. *)
+(* Qed. *)
 
-#[local]
-  Hint Resolve presup_exp_eq_natrec_cong_right : mcpts.
-
-
-Lemma presup_exp_eq_natrec_sub_left {P} : forall {Γ : ctx P}  {σ Δ A MZ MS M s s'} {r : Ru_nat P s},
-    {{ ⊢ Γ }} ->
-    {{ ⊢ Δ }} ->
-    {{ Γ ⊢s σ : Δ }} ->
-    {{ ⊢ Δ, ℕ }} ->
-    {{ Δ, ℕ ⊢ A : Sort@s' }} ->
-    {{ Δ ⊢ MZ : A[Id,,zero] }} ->
-    {{ ⊢ Δ, ℕ, A }} ->
-    {{ Δ, ℕ, A ⊢ MS : A[Wk∘Wk,,succ #1] }} ->
-    {{ Δ ⊢ M : ℕ }} ->
-    {{ Γ ⊢ rec M return A | zero -> MZ | succ -> MS end[σ] : A[σ,,M[σ]] }}.
-Proof.
-  intros.
-  assert {{ Δ, ℕ ⊢ A }} by mauto 2.
-  assert {{ Γ ⊢s σ,,M[σ] : Δ, ℕ }} by mauto 3.
-  assert {{ Γ ⊢ A[σ,,M[σ]] }} by mauto 2.
-  assert {{ Δ ⊢s Id,,M : Δ, ℕ }} by mauto 3.
-  assert {{ Γ ⊢s (Id,,M)∘σ ≈ σ,,M[σ] : Δ, ℕ }} by mauto.
-  assert {{ Γ ⊢ A[(Id,,M)∘σ] ≈ A[σ,,M[σ]] }} by mauto 3.
-  assert {{ Γ ⊢ A[Id,,M][σ] ≈ A[σ,,M[σ]] }} by mauto 3.
-  eapply wf_conv; mauto 3.
-Qed.
-
-#[local]
-  Hint Resolve presup_exp_eq_natrec_sub_left : mcpts.
+(* #[local] *)
+(*   Hint Resolve presup_exp_eq_natrec_cong_right : mcpts. *)
 
 
+(* Lemma presup_exp_eq_natrec_sub_left {P} : forall {Γ : ctx P}  {σ Δ A MZ MS M s s'} {r : Ru_nat P s}, *)
+(*     {{ ⊢ Γ }} -> *)
+(*     {{ ⊢ Δ }} -> *)
+(*     {{ Γ ⊢s σ : Δ }} -> *)
+(*     {{ ⊢ Δ, ℕ }} -> *)
+(*     {{ Δ, ℕ ⊢ A : Sort@s' }} -> *)
+(*     {{ Δ ⊢ MZ : A[Id,,zero] }} -> *)
+(*     {{ ⊢ Δ, ℕ, A }} -> *)
+(*     {{ Δ, ℕ, A ⊢ MS : A[Wk∘Wk,,succ #1] }} -> *)
+(*     {{ Δ ⊢ M : ℕ }} -> *)
+(*     {{ Γ ⊢ rec M return A | zero -> MZ | succ -> MS end[σ] : A[σ,,M[σ]] }}. *)
+(* Proof. *)
+(*   intros. *)
+(*   assert {{ Δ, ℕ ⊢ A }} by mauto 2. *)
+(*   assert {{ Γ ⊢s σ,,M[σ] : Δ, ℕ }} by mauto 3. *)
+(*   assert {{ Γ ⊢ A[σ,,M[σ]] }} by mauto 2. *)
+(*   assert {{ Δ ⊢s Id,,M : Δ, ℕ }} by mauto 3. *)
+(*   assert {{ Γ ⊢s (Id,,M)∘σ ≈ σ,,M[σ] : Δ, ℕ }} by mauto. *)
+(*   assert {{ Γ ⊢ A[(Id,,M)∘σ] ≈ A[σ,,M[σ]] }} by mauto 3. *)
+(*   assert {{ Γ ⊢ A[Id,,M][σ] ≈ A[σ,,M[σ]] }} by mauto 3. *)
+(*   eapply wf_conv; mauto 3. *)
+(* Qed. *)
 
-Lemma presup_exp_eq_natrec_sub_right {P} : forall {Γ : ctx P} {σ Δ A MZ MS M s s'} {r : Ru_nat P s},
-    {{ ⊢ Γ }} ->
-    {{ ⊢ Δ }} ->
-    {{ Γ ⊢s σ : Δ }} ->
-    {{ ⊢ Δ, ℕ }} ->
-    {{ Δ, ℕ ⊢ A : Sort@s' }} ->
-    {{ Δ ⊢ MZ : A[Id,,zero] }} ->
-    {{ ⊢ Δ, ℕ, A }} ->
-    {{ Δ, ℕ, A ⊢ MS : A[Wk∘Wk,,succ #1] }} ->
-    {{ Δ ⊢ M : ℕ }} ->
-    {{ Γ ⊢ rec M[σ] return A[q σ] | zero -> MZ[σ] | succ -> MS[q (q σ)] end : A[σ,,M[σ]] }}.
-Proof.
-  intros.
-  assert {{ Δ, ℕ ⊢ A }} by mauto 2.
-  assert {{ Γ, ℕ ⊢s q σ : Δ, ℕ }} by mauto 2.
-  assert {{ Γ, ℕ, A[q σ] ⊢s q (q σ) : Δ, ℕ, A }} by mauto 2.
-  assert {{ Γ, ℕ ⊢ A[q σ] }} by mauto 3.
-  (* Possible lemma? *)
-  assert (forall N, {{ Γ ⊢ N : ℕ }} -> {{ Γ ⊢ A[q σ][Id,,N] }} /\ {{ Γ ⊢ A[q σ][Id,,N] ≈ A[σ,,N] }}).
-  {
-    intros.
-    assert {{ Γ ⊢ N : ℕ[σ] }} by mauto 3.
-    assert {{ Γ ⊢s Id,,N : Γ, ℕ }} by mauto 3.
-    assert {{ Γ ⊢s q σ∘(Id,,N) ≈ σ,,N : Δ, ℕ }} by mauto 3.
-    assert {{ Γ ⊢s σ,,N : Δ, ℕ }} by mauto 2.
-    assert {{ Γ ⊢ A[q σ∘(Id,,N)] ≈ A[σ,,N] }} by mauto 3.
-    split; mauto 3.
-  }
-  (* Assertion for M *)
-  assert {{ Γ ⊢ M[σ] : ℕ }} by mauto 3.
-  (* Assertion for type *)
-  assert ({{ Γ ⊢ A[q σ][Id,,M[σ]] }} /\ {{ Γ ⊢ A[q σ][Id,,M[σ]] ≈ A[σ,,M[σ]] }}) as [] by mauto 3.
-   (* Assertion for MZ *)
-  assert {{ Δ ⊢ zero : ℕ }} by mauto 2.
-  assert {{ Δ ⊢s Id,,zero : Δ, ℕ }} by mauto.
-  assert {{ Γ ⊢ zero[σ] ≈ zero : ℕ }} by mauto 2.
-  assert {{ Γ ⊢s σ,,zero[σ] ≈ σ,,zero : Δ, ℕ }} by mauto 3.
-  assert {{ Γ ⊢s (Id,,zero)∘σ ≈ σ,,zero : Δ, ℕ }} by mauto.
-  assert ({{ Γ ⊢ A[q σ][Id,,zero] }} /\ {{ Γ ⊢ A[q σ][Id,,zero] ≈ A[σ,,zero] }}) as [] by mauto 3.
-  assert {{ Γ ⊢ A[(Id,,zero)∘σ] ≈ A[σ,,zero] }} by mauto 3.
-  assert {{ Γ ⊢ A[q σ][Id,,zero] ≈ A[Id,,zero][σ] }} by (etransitivity; [| symmetry]; mauto 3).
-  assert {{ Γ ⊢ MZ[σ] : A[q σ][Id,,zero] }} by mauto 4.
-  (* Assertion for MS *)
-  assert {{ Δ, ℕ, A ⊢s Wk∘Wk,,succ #1 : Δ, ℕ }}  by (eapply @sub_weak_compose_weak_extend_succ_var_1 with (P := P); mauto). 
-  assert {{ Γ, ℕ, A[q σ] ⊢s Wk∘Wk,,succ #1 : Γ, ℕ }}  by (eapply @sub_weak_compose_weak_extend_succ_var_1 with (P := P); mauto). 
-  assert {{ Γ, ℕ, A[q σ] ⊢s q σ∘(Wk∘Wk,,succ #1) ≈ (Wk∘Wk,,succ #1)∘q (q σ) : Δ, ℕ }} by mauto 2.
-  assert {{ Γ, ℕ, A[q σ] ⊢ A[q σ][Wk∘Wk,,succ #1] ≈ A[Wk∘Wk,,succ #1][q (q σ)] }} by mauto 2.
-  assert {{ Γ, ℕ, A[q σ] ⊢ MS[q (q σ)] : A[q σ][Wk∘Wk,,succ #1] }} by (eapply wf_conv; mauto 2).
-  (* Final *)
-  eapply wf_conv; mauto 3.
-Qed.
-
-#[local]
-Hint Resolve presup_exp_eq_natrec_sub_right : mcpts.
+(* #[local] *)
+(*   Hint Resolve presup_exp_eq_natrec_sub_left : mcpts. *)
 
 
-Lemma presup_exp_eq_beta_succ_right {P} : forall {Γ : ctx P} {A MZ MS M s s'} {r : Ru_nat P s},
-    {{ ⊢ Γ, ℕ }} ->
-    {{ Γ, ℕ ⊢ A : Sort@s' }} ->
-    {{ ⊢ Γ }} ->
-    {{ Γ ⊢ MZ : A[Id,,zero] }} ->
-    {{ ⊢ Γ, ℕ, A }} ->
-    {{ Γ, ℕ, A ⊢ MS : A[Wk∘Wk,,succ #1] }} ->
-    {{ Γ ⊢ M : ℕ }} ->
-    {{ Γ ⊢ MS[Id,,M,,rec M return A | zero -> MZ | succ -> MS end] : A[Id,,succ M] }}.
-Proof.
-  intros.
-  assert {{ Γ, ℕ ⊢ A }} by mauto 2.
-  (** Coq was having trouble inferring P here, expanded definition for now **)
-  (** set (WkWksucc := {{{ Wk∘Wk,,succ #1 }}}). **)
-  set (recM := {{{ rec M return A | zero -> MZ | succ -> MS end }}}).
-  set (IdMrecM := {{{ Id,,M,,recM }}}).
-  (* Assertion for type *)
-  assert {{ Γ ⊢ ℕ  }} by mauto 3.
-  assert {{ Γ ⊢ recM : A[Id,,M] }} by mauto 4.
-  assert {{ Γ, ℕ ⊢s Wk : Γ }} by mauto 2.
-  assert {{ Γ, ℕ, A ⊢s Wk : Γ, ℕ }} by mauto 2.
-  assert {{ Γ, ℕ, A ⊢s Wk∘Wk : Γ }} by mauto 2.
-  assert {{ Γ ⊢s (Wk∘Wk,,succ #1)∘IdMrecM ≈ (Wk∘Wk)∘IdMrecM,,(succ #1)[IdMrecM] : Γ, ℕ }}
-    by (eapply @sub_eq_extend_compose_nat with (P := P); mauto 4).
-  assert {{ Γ ⊢s Id : Γ }} by mauto 2.
-  assert {{ Γ ⊢s IdMrecM : Γ, ℕ, A }} by mauto 3.
-  assert {{ Γ ⊢s (Wk∘Wk)∘IdMrecM : Γ }} by mauto 2.
-  assert {{ Γ ⊢s (Wk∘Wk)∘IdMrecM ≈ Wk∘(Wk∘IdMrecM) : Γ }} by mauto 2.
-  assert {{ Γ ⊢s Id,,M : Γ, ℕ }} by mauto 2.
-  assert {{ Γ ⊢s Wk∘(Wk∘IdMrecM) ≈ Wk∘(Id,,M) : Γ }} by (econstructor; mauto 2).
-  assert {{ Γ ⊢s (Wk∘Wk)∘IdMrecM ≈ Id : Γ }} by (etransitivity; mauto 3).
-  assert {{ Γ ⊢ #1[IdMrecM] ≈ #0[Id,,M] : ℕ }} by mauto 3.
-  assert {{ Γ ⊢ #1[IdMrecM] ≈ M : ℕ }} by mauto 3.
-  assert {{ Γ ⊢ succ #1[IdMrecM] ≈ succ M : ℕ }} by mauto 2.
-  assert {{ Γ ⊢ (succ #1)[IdMrecM] ≈ succ M : ℕ }} by (etransitivity; mauto 3).
-  assert {{ Γ ⊢s (Wk∘Wk)∘IdMrecM,,(succ #1)[IdMrecM] ≈ Id,,succ M : Γ, ℕ }} by mauto 2.
-  assert {{ Γ ⊢s (Wk∘Wk,,succ #1)∘IdMrecM : Γ, ℕ }} by mauto 5.
-  assert {{ Γ ⊢s Id,,succ M : Γ, ℕ }} by mauto 3.
-  assert {{ Γ ⊢s (Wk∘Wk,,succ #1)∘IdMrecM ≈ Id,,succ M : Γ, ℕ }} by mauto 2.
-  assert {{ Γ ⊢ A[(Wk∘Wk,,succ #1)∘IdMrecM] ≈ A[Id,,succ M] }} by mauto.
-  enough {{ Γ ⊢ A[Wk∘Wk,,succ #1][IdMrecM] ≈ A[Id,,succ M] }}; [eapply wf_conv | etransitivity]; mauto 5.
-Qed.
 
-#[local]
-  Hint Resolve presup_exp_eq_beta_succ_right :
-  mcpts.
+(* Lemma presup_exp_eq_natrec_sub_right {P} : forall {Γ : ctx P} {σ Δ A MZ MS M s s'} {r : Ru_nat P s}, *)
+(*     {{ ⊢ Γ }} -> *)
+(*     {{ ⊢ Δ }} -> *)
+(*     {{ Γ ⊢s σ : Δ }} -> *)
+(*     {{ ⊢ Δ, ℕ }} -> *)
+(*     {{ Δ, ℕ ⊢ A : Sort@s' }} -> *)
+(*     {{ Δ ⊢ MZ : A[Id,,zero] }} -> *)
+(*     {{ ⊢ Δ, ℕ, A }} -> *)
+(*     {{ Δ, ℕ, A ⊢ MS : A[Wk∘Wk,,succ #1] }} -> *)
+(*     {{ Δ ⊢ M : ℕ }} -> *)
+(*     {{ Γ ⊢ rec M[σ] return A[q σ] | zero -> MZ[σ] | succ -> MS[q (q σ)] end : A[σ,,M[σ]] }}. *)
+(* Proof. *)
+(*   intros. *)
+(*   assert {{ Δ, ℕ ⊢ A }} by mauto 2. *)
+(*   assert {{ Γ, ℕ ⊢s q σ : Δ, ℕ }} by mauto 2. *)
+(*   assert {{ Γ, ℕ, A[q σ] ⊢s q (q σ) : Δ, ℕ, A }} by mauto 2. *)
+(*   assert {{ Γ, ℕ ⊢ A[q σ] }} by mauto 3. *)
+(*   (* Possible lemma? *) *)
+(*   assert (forall N, {{ Γ ⊢ N : ℕ }} -> {{ Γ ⊢ A[q σ][Id,,N] }} /\ {{ Γ ⊢ A[q σ][Id,,N] ≈ A[σ,,N] }}). *)
+(*   { *)
+(*     intros. *)
+(*     assert {{ Γ ⊢ N : ℕ[σ] }} by mauto 3. *)
+(*     assert {{ Γ ⊢s Id,,N : Γ, ℕ }} by mauto 3. *)
+(*     assert {{ Γ ⊢s q σ∘(Id,,N) ≈ σ,,N : Δ, ℕ }} by mauto 3. *)
+(*     assert {{ Γ ⊢s σ,,N : Δ, ℕ }} by mauto 2. *)
+(*     assert {{ Γ ⊢ A[q σ∘(Id,,N)] ≈ A[σ,,N] }} by mauto 3. *)
+(*     split; mauto 3. *)
+(*   } *)
+(*   (* Assertion for M *) *)
+(*   assert {{ Γ ⊢ M[σ] : ℕ }} by mauto 3. *)
+(*   (* Assertion for type *) *)
+(*   assert ({{ Γ ⊢ A[q σ][Id,,M[σ]] }} /\ {{ Γ ⊢ A[q σ][Id,,M[σ]] ≈ A[σ,,M[σ]] }}) as [] by mauto 3. *)
+(*    (* Assertion for MZ *) *)
+(*   assert {{ Δ ⊢ zero : ℕ }} by mauto 2. *)
+(*   assert {{ Δ ⊢s Id,,zero : Δ, ℕ }} by mauto. *)
+(*   assert {{ Γ ⊢ zero[σ] ≈ zero : ℕ }} by mauto 2. *)
+(*   assert {{ Γ ⊢s σ,,zero[σ] ≈ σ,,zero : Δ, ℕ }} by mauto 3. *)
+(*   assert {{ Γ ⊢s (Id,,zero)∘σ ≈ σ,,zero : Δ, ℕ }} by mauto. *)
+(*   assert ({{ Γ ⊢ A[q σ][Id,,zero] }} /\ {{ Γ ⊢ A[q σ][Id,,zero] ≈ A[σ,,zero] }}) as [] by mauto 3. *)
+(*   assert {{ Γ ⊢ A[(Id,,zero)∘σ] ≈ A[σ,,zero] }} by mauto 3. *)
+(*   assert {{ Γ ⊢ A[q σ][Id,,zero] ≈ A[Id,,zero][σ] }} by (etransitivity; [| symmetry]; mauto 3). *)
+(*   assert {{ Γ ⊢ MZ[σ] : A[q σ][Id,,zero] }} by mauto 4. *)
+(*   (* Assertion for MS *) *)
+(*   assert {{ Δ, ℕ, A ⊢s Wk∘Wk,,succ #1 : Δ, ℕ }}  by (eapply @sub_weak_compose_weak_extend_succ_var_1 with (P := P); mauto).  *)
+(*   assert {{ Γ, ℕ, A[q σ] ⊢s Wk∘Wk,,succ #1 : Γ, ℕ }}  by (eapply @sub_weak_compose_weak_extend_succ_var_1 with (P := P); mauto).  *)
+(*   assert {{ Γ, ℕ, A[q σ] ⊢s q σ∘(Wk∘Wk,,succ #1) ≈ (Wk∘Wk,,succ #1)∘q (q σ) : Δ, ℕ }} by mauto 2. *)
+(*   assert {{ Γ, ℕ, A[q σ] ⊢ A[q σ][Wk∘Wk,,succ #1] ≈ A[Wk∘Wk,,succ #1][q (q σ)] }} by mauto 2. *)
+(*   assert {{ Γ, ℕ, A[q σ] ⊢ MS[q (q σ)] : A[q σ][Wk∘Wk,,succ #1] }} by (eapply wf_conv; mauto 2). *)
+(*   (* Final *) *)
+(*   eapply wf_conv; mauto 3. *)
+(* Qed. *)
+
+(* #[local] *)
+(* Hint Resolve presup_exp_eq_natrec_sub_right : mcpts. *)
+
+
+(* Lemma presup_exp_eq_beta_succ_right {P} : forall {Γ : ctx P} {A MZ MS M s s'} {r : Ru_nat P s}, *)
+(*     {{ ⊢ Γ, ℕ }} -> *)
+(*     {{ Γ, ℕ ⊢ A : Sort@s' }} -> *)
+(*     {{ ⊢ Γ }} -> *)
+(*     {{ Γ ⊢ MZ : A[Id,,zero] }} -> *)
+(*     {{ ⊢ Γ, ℕ, A }} -> *)
+(*     {{ Γ, ℕ, A ⊢ MS : A[Wk∘Wk,,succ #1] }} -> *)
+(*     {{ Γ ⊢ M : ℕ }} -> *)
+(*     {{ Γ ⊢ MS[Id,,M,,rec M return A | zero -> MZ | succ -> MS end] : A[Id,,succ M] }}. *)
+(* Proof. *)
+(*   intros. *)
+(*   assert {{ Γ, ℕ ⊢ A }} by mauto 2. *)
+(*   (** Coq was having trouble inferring P here, expanded definition for now **) *)
+(*   (** set (WkWksucc := {{{ Wk∘Wk,,succ #1 }}}). **) *)
+(*   set (recM := {{{ rec M return A | zero -> MZ | succ -> MS end }}}). *)
+(*   set (IdMrecM := {{{ Id,,M,,recM }}}). *)
+(*   (* Assertion for type *) *)
+(*   assert {{ Γ ⊢ ℕ  }} by mauto 3. *)
+(*   assert {{ Γ ⊢ recM : A[Id,,M] }} by mauto 4. *)
+(*   assert {{ Γ, ℕ ⊢s Wk : Γ }} by mauto 2. *)
+(*   assert {{ Γ, ℕ, A ⊢s Wk : Γ, ℕ }} by mauto 2. *)
+(*   assert {{ Γ, ℕ, A ⊢s Wk∘Wk : Γ }} by mauto 2. *)
+(*   assert {{ Γ ⊢s (Wk∘Wk,,succ #1)∘IdMrecM ≈ (Wk∘Wk)∘IdMrecM,,(succ #1)[IdMrecM] : Γ, ℕ }} *)
+(*     by (eapply @sub_eq_extend_compose_nat with (P := P); mauto 4). *)
+(*   assert {{ Γ ⊢s Id : Γ }} by mauto 2. *)
+(*   assert {{ Γ ⊢s IdMrecM : Γ, ℕ, A }} by mauto 3. *)
+(*   assert {{ Γ ⊢s (Wk∘Wk)∘IdMrecM : Γ }} by mauto 2. *)
+(*   assert {{ Γ ⊢s (Wk∘Wk)∘IdMrecM ≈ Wk∘(Wk∘IdMrecM) : Γ }} by mauto 2. *)
+(*   assert {{ Γ ⊢s Id,,M : Γ, ℕ }} by mauto 2. *)
+(*   assert {{ Γ ⊢s Wk∘(Wk∘IdMrecM) ≈ Wk∘(Id,,M) : Γ }} by (econstructor; mauto 2). *)
+(*   assert {{ Γ ⊢s (Wk∘Wk)∘IdMrecM ≈ Id : Γ }} by (etransitivity; mauto 3). *)
+(*   assert {{ Γ ⊢ #1[IdMrecM] ≈ #0[Id,,M] : ℕ }} by mauto 3. *)
+(*   assert {{ Γ ⊢ #1[IdMrecM] ≈ M : ℕ }} by mauto 3. *)
+(*   assert {{ Γ ⊢ succ #1[IdMrecM] ≈ succ M : ℕ }} by mauto 2. *)
+(*   assert {{ Γ ⊢ (succ #1)[IdMrecM] ≈ succ M : ℕ }} by (etransitivity; mauto 3). *)
+(*   assert {{ Γ ⊢s (Wk∘Wk)∘IdMrecM,,(succ #1)[IdMrecM] ≈ Id,,succ M : Γ, ℕ }} by mauto 2. *)
+(*   assert {{ Γ ⊢s (Wk∘Wk,,succ #1)∘IdMrecM : Γ, ℕ }} by mauto 5. *)
+(*   assert {{ Γ ⊢s Id,,succ M : Γ, ℕ }} by mauto 3. *)
+(*   assert {{ Γ ⊢s (Wk∘Wk,,succ #1)∘IdMrecM ≈ Id,,succ M : Γ, ℕ }} by mauto 2. *)
+(*   assert {{ Γ ⊢ A[(Wk∘Wk,,succ #1)∘IdMrecM] ≈ A[Id,,succ M] }} by mauto. *)
+(*   enough {{ Γ ⊢ A[Wk∘Wk,,succ #1][IdMrecM] ≈ A[Id,,succ M] }}; [eapply wf_conv | etransitivity]; mauto 5. *)
+(* Qed. *)
+
+(* #[local] *)
+(*   Hint Resolve presup_exp_eq_beta_succ_right : *)
+(*   mcpts. *)
 
 
 #[local]
