mechanization/theories/Core/Syntactic/Syntax.v
@@ -3,51 +3,51 @@ From Coq Require Import List String.
 From McPTS Require Import PtsSignature.
 From McPTS.Core Require Import Base.
 
-
+(* This is needed for frontend, which we don't cover *)
 (** * Concrete Syntax Tree *)
-Module Cst.
-  Inductive obj (P : PtsSig) : Set :=
-  (** Sorts *)
-  | st : P -> obj P
-  (** Functions *)
-  | pi : string -> obj P -> obj P -> obj P
-  | fn : string -> obj P -> obj P -> obj P
-  | app : obj P -> obj P -> obj P
-  (** Variables *)
-  | var : string -> obj P
-  (** Naturals **)
-  | nat : obj P
-  | zero : obj P
-  | succ : obj P -> obj P
-  | natrec : obj P -> string -> obj P -> obj P -> string -> string -> obj P -> obj P.
-  Arguments st {_}.
-  Arguments pi {_}.
-  Arguments fn {_}.
-  Arguments app {_}.
-  Arguments nat {_}.
-  Arguments zero {_}.
-  Arguments succ {_}.
-  Arguments natrec {_}.
-  Arguments var {_}.
-End Cst.
+(* Module Cst. *)
+(*   Inductive obj (P : PtsSig) : Set := *)
+(*   (** Sorts *) *)
+(*   | st : P -> obj P *)
+(*   (** Functions *) *)
+(*   | pi : string -> obj P -> obj P -> obj P *)
+(*   | fn : string -> obj P -> obj P -> obj P *)
+(*   | app : obj P -> obj P -> obj P *)
+(*   (** Variables *) *)
+(*   | var : string -> obj P *)
+(*   (** Naturals **) *)
+(*   | nat : obj P *)
+(*   | zero : obj P *)
+(*   | succ : obj P -> obj P *)
+(*   | natrec : obj P -> string -> obj P -> obj P -> string -> string -> obj P -> obj P. *)
+(*   Arguments st {_}. *)
+(*   Arguments pi {_}. *)
+(*   Arguments fn {_}. *)
+(*   Arguments app {_}. *)
+(*   Arguments nat {_}. *)
+(*   Arguments zero {_}. *)
+(*   Arguments succ {_}. *)
+(*   Arguments natrec {_}. *)
+(*   Arguments var {_}. *)
+(* End Cst. *)
 
 (** * Abstract Syntax Tree *)
 Inductive exp (P : PtsSig) : Set :=
 (** Sorts *)
 | a_st : P -> exp P
 (** Functions *)
-| a_pi : forall (s1 s2 s3 : P), Ru P s1 s2 s3 -> exp P -> exp P -> exp P
-| a_fn : forall (s1 s2 s3 : P), Ru P s1 s2 s3 -> exp P -> exp P -> exp P
+| a_pi : exp P -> exp P -> exp P
+| a_fn : exp P -> exp P -> exp P
 | a_app : exp P -> exp P -> exp P
 (** Variable *)
 | a_var : nat -> exp P
 (** Substitution Application *)
 | a_sub : exp P -> sub P -> exp P
 (** Naturals **)
-| a_nat : exp P
-| a_zero : exp P
-| a_succ : exp P -> exp P
-| a_natrec : exp P -> exp P -> exp P -> exp P -> exp P
+(* | a_nat : exp P *)
+(* | a_zero : exp P *)
+(* | a_succ : exp P -> exp P *)
+(* | a_natrec : exp P -> exp P -> exp P -> exp P -> exp P *)
 with sub (P : PtsSig) : Set :=
 | a_id : sub P
 | a_weaken : sub P
@@ -55,15 +55,15 @@ with sub (P : PtsSig) : Set :=
 | a_extend : sub P -> exp P -> sub P.
 
 Arguments a_st {_}.
-Arguments a_pi {_ _ _ _}.
-Arguments a_fn {_ _ _ _}.
+Arguments a_pi {_}.
+Arguments a_fn {_}.
 Arguments a_app {_}.
 Arguments a_var {_}.
 Arguments a_sub {_}.
-Arguments a_nat {_}.
-Arguments a_zero {_}.
-Arguments a_succ {_}.
-Arguments a_natrec {_}.
+(* Arguments a_nat {_}. *)
+(* Arguments a_zero {_}. *)
+(* Arguments a_succ {_}. *)
+(* Arguments a_natrec {_}. *)
 Arguments a_id {_}.
 Arguments a_weaken {_}.
 Arguments a_compose {_}.
@@ -73,31 +73,31 @@ Arguments a_extend {_}.
 Notation typ := (fun P => exp P).
 Notation ctx := (fun P => list (typ P)).
 
-Fixpoint nat_to_exp {P : PtsSig} (n : nat) : exp P :=
-  match n with
-  | 0 => a_zero
-  | S m => a_succ (nat_to_exp m)
-  end.
+(* Fixpoint nat_to_exp {P : PtsSig} (n : nat) : exp P := *)
+(*   match n with *)
+(*   | 0 => a_zero *)
+(*   | S m => a_succ (nat_to_exp m) *)
+(*   end. *)
 
-Definition num_to_exp {P : PtsSig} (n : Number.uint) : exp P :=
-  nat_to_exp (Nat.of_num_uint n).
+(* Definition num_to_exp {P : PtsSig} (n : Number.uint) : exp P := *)
+(*   nat_to_exp (Nat.of_num_uint n). *)
 
-Fixpoint exp_to_nat {P : PtsSig} (e : exp P) : option nat :=
-  match e with
-  | a_zero => Some 0
-  | a_succ e' =>
-      match exp_to_nat e' with
-      | Some n => Some (S n)
-      | None => None
-      end
-  | _ => None
-  end.
+(* Fixpoint exp_to_nat {P : PtsSig} (e : exp P) : option nat := *)
+(*   match e with *)
+(*   | a_zero => Some 0 *)
+(*   | a_succ e' => *)
+(*       match exp_to_nat e' with *)
+(*       | Some n => Some (S n) *)
+(*       | None => None *)
+(*       end *)
+(*   | _ => None *)
+(*   end. *)
 
-Definition exp_to_num {P : PtsSig} (e : exp P) :=
-  match exp_to_nat e with
-  | Some n => Some (Nat.to_num_uint n)
-  | None => None
-  end.
+(* Definition exp_to_num {P : PtsSig} (e : exp P) := *)
+(*   match exp_to_nat e with *)
+(*   | Some n => Some (Nat.to_num_uint n) *)
+(*   | None => None *)
+(*   end. *)
 
 
 Scheme exp_mut_ind := Induction for exp Sort Prop
@@ -109,45 +109,45 @@ Combined Scheme syntax_mut_ind from
 (** ** Syntactic Normal/Neutral Form *)
 Inductive nf (P : PtsSig) : Set :=
 | nf_st : P -> nf P
-| nf_pi : forall (s1 s2 s3 : P), Ru P s1 s2 s3 -> nf P -> nf P -> nf P
-| nf_fn : forall (s1 s2 s3 : P), Ru P s1 s2 s3 -> nf P -> nf P -> nf P
-| nf_nat : nf P
-| nf_zero : nf P
-| nf_succ : nf P -> nf P
+| nf_pi : nf P -> nf P -> nf P
+| nf_fn : nf P -> nf P -> nf P
+(* | nf_nat : nf P *)
+(* | nf_zero : nf P *)
+(* | nf_succ : nf P -> nf P *)
 | nf_neut : ne P -> nf P
 with ne (P : PtsSig) : Set :=
 | ne_app : ne P -> nf P -> ne P
 | ne_var : nat -> ne P
-| ne_natrec : nf P -> nf P -> nf P -> ne P -> ne P
+(* | ne_natrec : nf P -> nf P -> nf P -> ne P -> ne P *)
 .
 
 Arguments nf_st {_}.
-Arguments nf_pi {_ _ _ _}.
-Arguments nf_fn {_ _ _ _}.
-Arguments nf_nat {_}.
-Arguments nf_zero {_}.
-Arguments nf_succ {_}.
+Arguments nf_pi {_}.
+Arguments nf_fn {_}.
+(* Arguments nf_nat {_}. *)
+(* Arguments nf_zero {_}. *)
+(* Arguments nf_succ {_}. *)
 Arguments nf_neut {_}.
 
 Arguments ne_app {_}.
 Arguments ne_var {_}.
-Arguments ne_natrec {_}.
+(* Arguments ne_natrec {_}. *)
 
 Fixpoint nf_to_exp {P : PtsSig} (M : nf P) : exp P :=
   match M with
   | nf_st s => a_st s
-  | nf_pi r A B => a_pi r (nf_to_exp A) (nf_to_exp B)
-  | nf_fn r A M => a_fn r (nf_to_exp A) (nf_to_exp M)
-  | nf_nat => a_nat
-  | nf_zero => a_zero
-  | nf_succ M => a_succ (nf_to_exp M)
+  | nf_pi A B => a_pi (nf_to_exp A) (nf_to_exp B)
+  | nf_fn A M => a_fn (nf_to_exp A) (nf_to_exp M)
+  (* | nf_nat => a_nat *)
+  (* | nf_zero => a_zero *)
+  (* | nf_succ M => a_succ (nf_to_exp M) *)
   | nf_neut M => ne_to_exp M
   end
 with ne_to_exp {P : PtsSig} (M : ne P) : exp P :=
   match M with
   | ne_app M N => a_app (ne_to_exp M) (nf_to_exp N)
   | ne_var x => a_var x
-  | ne_natrec A MZ MS M => a_natrec (nf_to_exp A) (nf_to_exp MZ) (nf_to_exp MS) (ne_to_exp M)
+  (* | ne_natrec A MZ MS M => a_natrec (nf_to_exp A) (nf_to_exp MZ) (nf_to_exp MS) (ne_to_exp M) *)
   end
 .
 
@@ -188,12 +188,12 @@ Module Syntax_Notations.
   Notation "x" := x (in custom exp at level 0, x ident) : mcpts_scope.
 
   Notation "'Sort' @ s" := (a_st s) (in custom exp at level 0, s constr at level 0, format "'Sort' @ s") : mcpts_scope.
-  Notation "'ℕ'" := a_nat (in custom exp at level 0) : mcpts_scope.
-  Notation "'zero'" := a_zero (in custom exp at level 0) : mcpts_scope.
-  Notation "'succ' e" := (a_succ e) (in custom exp at level 1, e custom exp at level 0) : mcpts_scope.
-  Notation "'rec' e 'return' A | 'zero' -> ez | 'succ' -> es 'end'" := (a_natrec A ez es e) (in custom exp at level 0, A custom exp at level 60, ez custom exp at level 60, es custom exp at level 60, e custom exp at level 60) : mcpts_scope.
-  Notation "'Π' r A B" := (a_pi r A B) (in custom exp at level 1, r constr at level 0, A custom exp at level 0, B custom exp at level 60) : mcpts_scope.
-  Notation "'λ' r A e" := (a_fn r A e) (in custom exp at level 1, r constr at level 0, A custom exp at level 0, e custom exp at level 60) : mcpts_scope.
+  (* Notation "'ℕ'" := a_nat (in custom exp at level 0) : mcpts_scope. *)
+  (* Notation "'zero'" := a_zero (in custom exp at level 0) : mcpts_scope. *)
+  (* Notation "'succ' e" := (a_succ e) (in custom exp at level 1, e custom exp at level 0) : mcpts_scope. *)
+  (* Notation "'rec' e 'return' A | 'zero' -> ez | 'succ' -> es 'end'" := (a_natrec A ez es e) (in custom exp at level 0, A custom exp at level 60, ez custom exp at level 60, es custom exp at level 60, e custom exp at level 60) : mcpts_scope. *)
+  Notation "'Π' A B" := (a_pi A B) (in custom exp at level 1, A custom exp at level 0, B custom exp at level 60) : mcpts_scope.
+  Notation "'λ' A e" := (a_fn A e) (in custom exp at level 1, A custom exp at level 0, e custom exp at level 60) : mcpts_scope.
   Notation "f x .. y" := (a_app .. (a_app f x) .. y) (in custom exp at level 40, f custom exp, x custom exp at next level, y custom exp at next level) : mcpts_scope.
   Notation "'#' n" := (a_var n) (in custom exp at level 0, n constr at level 0, format "'#' n") : mcpts_scope.
 
@@ -212,12 +212,12 @@ Module Syntax_Notations.
   Notation "x" := x (in custom nf at level 0, x ident) : mcpts_scope.
 
   Notation "'Sort' @ s" := (nf_st s) (in custom nf at level 0, s constr at level 0, format "'Sort' @ s") : mcpts_scope.
-  Notation "'ℕ'" := nf_nat (in custom nf at level 0) : mcpts_scope.
-  Notation "'zero'" := nf_zero (in custom nf at level 0) : mcpts_scope.
-  Notation "'succ' M" := (nf_succ M) (in custom nf at level 2, M custom nf at level 1) : mcpts_scope.
-  Notation "'rec' M 'return' A | 'zero' -> MZ | 'succ' -> MS 'end'" := (ne_natrec A MZ MS M) (in custom nf at level 0, A custom nf at level 60, MZ custom nf at level 60, MS custom nf at level 60, M custom nf at level 60) : mcpts_scope.
-  Notation "'Π' r A B" := (nf_pi r A B) (in custom nf at level 2, r constr at level 0, A custom nf at level 1, B custom nf at level 60) : mcpts_scope.
-  Notation "'λ' r A e" := (nf_fn r A e) (in custom nf at level 2, r constr at level 0, A custom nf at level 1, e custom nf at level 60) : mcpts_scope.
+  (* Notation "'ℕ'" := nf_nat (in custom nf at level 0) : mcpts_scope. *)
+  (* Notation "'zero'" := nf_zero (in custom nf at level 0) : mcpts_scope. *)
+  (* Notation "'succ' M" := (nf_succ M) (in custom nf at level 2, M custom nf at level 1) : mcpts_scope. *)
+  (* Notation "'rec' M 'return' A | 'zero' -> MZ | 'succ' -> MS 'end'" := (ne_natrec A MZ MS M) (in custom nf at level 0, A custom nf at level 60, MZ custom nf at level 60, MS custom nf at level 60, M custom nf at level 60) : mcpts_scope. *)
+  Notation "'Π' A B" := (nf_pi A B) (in custom nf at level 2, A custom nf at level 1, B custom nf at level 60) : mcpts_scope.
+  Notation "'λ' A e" := (nf_fn A e) (in custom nf at level 2, A custom nf at level 1, e custom nf at level 60) : mcpts_scope.
   Notation "f x .. y" := (ne_app .. (ne_app f x) .. y) (in custom nf at level 40, f custom nf, x custom nf at next level, y custom nf at next level) : mcpts_scope.
   Notation "'#' n" := (ne_var n) (in custom nf at level 0, n constr at level 0, format "'#' n") : mcpts_scope.
   Notation "'⇑' M" := (nf_neut M) (in custom nf at level 0, M custom nf at level 99, format "'⇑'  M") : mcpts_scope.
